\documentclass[10pt,a4paper, margin=1in]{article}
\usepackage{fullpage}
\usepackage{amsfonts, amsmath, pifont}
\usepackage{amsthm}
\usepackage{graphicx}

\usepackage{geometry}
 \geometry{
 a4paper,
 total={210mm,297mm},
 left=10mm,
 right=10mm,
 top=10mm,
 bottom=10mm,
 }
 % Write both of your names here. Fill exxxxxxx with your ceng mail address.
 \author{
  KASAP, Åžahin\\
  \texttt{e2264562@ceng.metu.edu.tr}
  \and
  US, Muhammed Beyhan\\
  \texttt{e2264711@ceng.metu.edu.tr}
}
\title{CENG 384 - Signals and Systems for Computer Engineers \\
Spring 2018-2019 \\
Written Assignment 4}
\begin{document}
\maketitle



\noindent\rule{19cm}{1.2pt}

\begin{enumerate}

\item 
    \begin{enumerate}
    % Write your solutions in the following items.
    \item %write the solution of q1a
	$ y[n]- \frac{3}{4}y[n-1]+\frac{1}{8}y[n-2]=2x[n] $ \\
	$ $ \\

    \item %write the solution of q1b
	$H(e^{jw})=\frac{2}{1-\frac{3}{4}e^{-jw}+\frac{1}{8}e^{-2jw}} $ \\
    $ $ \\



    \item %write the solution of q1c
    $H(e^{jw})=\frac{2}{(1-\frac{1}{2}e^{-jw})(1-\frac{1}{4}e^{-jw})} $ \\
    $H(e^{jw})= \frac{4}{1-\frac{1}{2}e^{-jw}}-\frac{2}{1-\frac{1}{4}e^{-jw}} $ \\
        $ $ \\


    $\Rightarrow h[n]=4(\frac{1}{2})^nu[n]-2(\frac{1}{4})^nu[n] $ \\
    $ $ \\


    \item %write the solution of q1d
    $X(e^{jw})=\frac{1}{1-\frac{1}{4}e^{-jw}} $ \\
	$Y(e^{jw})=H(e^{jw})X(e^{jw}) $ \\
    $=\frac{2}{(1-\frac{1}{2}e^{-jw})(1-\frac{1}{4}e^{-jw})^2} $ \\
	$=-\frac{4}{1-\frac{1}{4}e^{-jw}}-\frac{2}{(1-\frac{1}{4}e^{-jw})^2}+\frac{8}{1-\frac{1}{2}e^{-jw}} $ \\
    $\Rightarrow y[n]=\lbrace -4(\frac{1}{4})^n-2(n+1)(\frac{1}{4})^n+8(\frac{1}{2})^n\rbrace u[n] $ \\
	$ $ \\
    $ $ \\
    
    \end{enumerate}


\item %write the solution of q2
	Because $h_{1}[n]$ and $4h_2[n]$ are connected in parallel  \\
	
    $h[n]=h_{1}[n] + h_2[n] $ \\
    Because it is LTI
    $\Rightarrow $\\
    $H[e^{jw}]=H_{1}[e^{jw}] + H_2[e^{jw}]  $ \\
    $ $ \\ It is given in the question that
    $ $ \\
    $H_{1}[e^{jw}]=\frac{1}{1-\frac{1}{3}e^{-jw}}  $ \\
	$H_{2}[e^{jw}]= H[e^{jw}]- H_{1}[e^{jw}]$ \\
    $H_{2}[e^{jw}]= \frac{5e^{-jw}-12}{e^{-2jw}-7e^{-jw}+12}- \frac{1}{1-\frac{1}{3}e^{-jw}} $ \\
	$ $ \\
    $ $ \\
	$ $ \\
    $ $ \\    

\item %write the solution of q3
    \begin{enumerate}
    \item %write the solution of q3a
    \item %write the solution of q3b
    \item %write the solution of q3c
    \end{enumerate}
\item %write the solution of q4
    \begin{enumerate}
    \item %write the solution of q4a
    \item %write the solution of q4b
    \item %write the solution of q4c
    \end{enumerate}
    
\end{enumerate}
\end{document}


